compiler/dsl/coq/ReflexDenoted.v
@@ -1,3 +1,19 @@
+Class SDenoted (T : Set) : Type :=
+{ sdenote : T -> Set
+}.
+Notation "s[[ x ]]" := (sdenote x).
+
+Definition optsdenote {T} `{SDenoted T} (ox : option T) :=
+  match ox with
+  | None => False
+  | Some x => s[[ x ]]
+  end.
+Notation "s[! x !]" := (optsdenote x).
+
+Instance SDenoted_option {T} `{ SDenoted T } : SDenoted (option T) :=
+{ sdenote := optsdenote
+}.
+
 Class Denoted (T : Type) : Type :=
 { denote : T -> Type
 }.
